src/Pact.v
@@ -1,19 +1,9 @@
-Require Import
-  Coq.Arith.Arith
-  Coq.ZArith.ZArith
-  Coq.micromega.Lia
-  Coq.Strings.String
-  Hask.Control.Monad
-  Data.Monoid
+Require Export
   Lib
-  Ltac
-  Ty
   Exp
+  SemTy
   Value
-  Sem
   RWSE.
-
-Set Universe Polymorphism.
 
 From Equations Require Import Equations.
 Set Equations With UIP.
@@ -21,115 +11,6 @@ Set Equations With UIP.
 Generalizable All Variables.
 
 Section Pact.
-
-Import ListNotations.
-
-Open Scope Ty_scope.
-
-Notation "⟦ t ⟧" := (SemTy t) (at level 9) : type_scope.
-
-(* This couldn't be derived due to the recursion at [VList]. *)
-Equations Decidable_EqDec (t : Ty) (H : DecidableP t) : EqDec ⟦t⟧ :=
-  Decidable_EqDec (TyPrim PrimUnit) _ tt tt := left _;
-  Decidable_EqDec (TyPair t1 t2) (PairDecP H1 H2) (x1, y1) (x2, y2)
-    with @eq_dec _ (Decidable_EqDec t1 H1) x1 x2 := {
-      | left  _ with @eq_dec _ (Decidable_EqDec t2 H2) y1 y2 := {
-        | left _  => left _
-        | right _ => right _
-      }
-      | right _ => right _
-  };
-  Decidable_EqDec (TyPrim PrimString) _ s1 s2
-    with eq_dec s1 s2 := {
-      | left _  => left _
-      | right _ => right _
-    };
-  Decidable_EqDec (TyPrim PrimInteger) _ i1 i2
-    with eq_dec i1 i2 := {
-      | left _  => left _
-      | right _ => right _
-    };
-  Decidable_EqDec (TyPrim PrimDecimal) _ d1 d2
-    with eq_dec d1 d2 := {
-      | left _  => left _
-      | right _ => right _
-    };
-  Decidable_EqDec (TyPrim PrimBool) _ b1 b2
-    with eq_dec b1 b2 := {
-      | left _  => left _
-      | right _ => right _
-    };
-  Decidable_EqDec (TyPrim PrimTime) _ t1 t2
-    with eq_dec t1 t2 := {
-      | left _  => left _
-      | right _ => right _
-    };
-  Decidable_EqDec (TyList _)  _ ([]) ([]) := left _;
-  Decidable_EqDec (TyList _)  _ (_ :: _) ([]) := right _;
-  Decidable_EqDec (TyList _)  _ ([]) (_ :: _) := right _;
-  Decidable_EqDec (TyList ty) (ListDecP H) (x1 :: xs1) (y1 :: ys1)
-    with @eq_dec _ (Decidable_EqDec ty H) x1 y1 := {
-      | left _
-        with @eq_dec _ (list_eqdec (Decidable_EqDec ty H)) xs1 ys1 := {
-        | left _  => left _
-        | right _ => right _
-      }
-      | right _ => right _
-    }.
-
-#[export]
-Instance Decidable_EqDec' {t} : DecidableP t → EqDec ⟦t⟧ :=
-  Decidable_EqDec t.
-
-Inductive Value {t} (D : DecidableP t) : Set :=
-  | Bundle : ⟦t⟧ → Value D.
-
-Derive NoConfusion NoConfusionHom Subterm for Value.
-
-#[export]
-Program Instance Value_EqDec {t} (D : DecidableP t) : EqDec (Value D).
-Next Obligation.
-  destruct x, y.
-  destruct (@eq_dec _ (Decidable_EqDec _ D) s s0); subst;
-  try (right; intro; inv H; contradiction);
-  now left.
-Defined.
-
-(******************************************************************************
- * The Pact environment
- *)
-
-(* (defcap TRANSFER (from:string to:string amount:decimal)
-      @managed amount TRANSFER_mgr
-      ...)
-
-   name    = "TRANSFER"
-   paramTy = (string × string)
-   valueTy = decimal
-*)
-
-Record CapSig : Set := {
-  name       : string;
-  paramTy    : Ty;              (* this could be a product (i.e. pair) *)
-  paramTyDec : DecidableP paramTy;
-  valueTy    : Ty;              (* TUnit for unmanaged caps *)
-  valueTyDec : DecidableP valueTy;
-}.
-
-Derive NoConfusion NoConfusionHom Subterm EqDec for CapSig.
-
-Inductive Cap `(s : CapSig) : Set :=
-  | Token : Value (paramTyDec s) → Value (valueTyDec s) → Cap s.
-
-Derive NoConfusion NoConfusionHom Subterm EqDec for Cap.
-
-Arguments Token {s} _.
-
-Definition paramOf `(c : Cap s) : Value (paramTyDec s) :=
-  match c with Token p _ => p end.
-
-Definition valueOf `(c : Cap s) : Value (valueTyDec s) :=
-  match c with Token _ v => v end.
 
 Inductive CapError : Set :=
   | CapErr_CapabilityNotAvailable
@@ -139,6 +20,7 @@ Inductive CapError : Set :=
 Derive NoConfusion NoConfusionHom Subterm EqDec for CapError.
 
 Inductive Err : Set :=
+  | Err_Exp : Exp.Err → Err
   | Err_Capability {s} : Cap s → CapError → Err.
 
 Derive NoConfusion NoConfusionHom Subterm EqDec for Err.
@@ -163,7 +45,7 @@ Record PactState : Set := {
   (* We cannot refer to capability tokens by their type here, because
      capability predicates execute in a state monad that reference this
      record type. *)
-  resources : list { s : CapSig & Cap s }
+  resources : list { s : CapSig & Cap s };
 }.
 
 Derive NoConfusion NoConfusionHom Subterm EqDec for PactState.
@@ -172,164 +54,6 @@ Record PactLog : Set := {}.
 
 Derive NoConfusion NoConfusionHom Subterm EqDec for PactLog.
 
-Definition PactM : Set → Set := @RWSE PactEnv PactState PactLog Err.
-
-(******************************************************************************
- * Capabilities
- *)
-
-Record DefCap `(s : CapSig) : Set := {
-  predicate : Cap s → PactM (list { s : CapSig & Cap s});
-  manager   : Value (valueTyDec s) → Value (valueTyDec s) →
-              PactM (Value (valueTyDec s))
-}.
-
-Derive NoConfusion NoConfusionHom Subterm for DefCap.
-
-Arguments predicate {s} _.
-Arguments manager {s} _.
-
-Import EqNotations.
-
-Definition get_value `(c : Cap s)
-           (l : list { k : CapSig & Cap k }) :
-  option (Value (valueTyDec s)) :=
-  let '(Token p _) := c in
-  let fix go (l : list {k : CapSig & Cap k}) :
-    option (Value (valueTyDec s)) :=
-    match l with
-    | [] => None
-    | existT _ s' (Token p' x') :: xs =>
-        match eq_dec s s' with
-        | left  Hs =>
-            match eq_dec p (rew <- [λ x, Value (paramTyDec x)] Hs in p') with
-            | left _ => Some (rew <- [λ x, Value (valueTyDec x)] Hs in x')
-            | _ => go xs
-            end
-        | _ => go xs
-        end
-    end
-  in go l.
-
-Definition set_value `(c : Cap s)
-           (l : list { k : CapSig & Cap k }) :
-  list { k : CapSig & Cap k } :=
-  let '(Token p _) := c in
-  let fix go (l : list {k : CapSig & Cap k}) :
-    list { k : CapSig & Cap k } :=
-    match l with
-    | [] => []
-    | existT _ s' (Token p' _) :: xs =>
-        match eq_dec s s' with
-        | left  Hs =>
-            match eq_dec p (rew <- [λ x, Value (paramTyDec x)] Hs in p') with
-            | left _ => existT _ s c :: go xs
-            | _ => go xs
-            end
-        | _ => go xs
-        end
-    end
-  in go l.
-
-(* The functions below all take a [DefCap] because name resolution must happen
-   in the parser, since capability predicates can themselves refer to the
-   current module. *)
-
-(* "Installing" a capability assigns a resource amount associated with that
-   capability, to be consumed by future calls to [with-capability].
-
-   Note that a capability can be installed either by the user calling
-   [install-capability] directly, or by the chain calling this function if it
-   sees a signed capability as part of a transaction. *)
-Definition install_capability `(D : DefCap s) (c : Cap s) : PactM () :=
-  env <- ask ;
-  if in_dec EvalContext_EqDec InWithCapability (context env)
-  then
-    throw (Err_Capability c CapErr_CannotInstallDuringWith)
-  else
-    modify (λ st, {| resources := set_value c (resources st) |}).
-
-Definition __claim_resource `(D : DefCap s) (c : Cap s) : PactM () :=
-  (* Check the current amount of resource associated with this capability, and
-     whether the requested amount is available. If so, update the available
-     amount. Note: unit is used to represent unmanaged capabilities. *)
-  if eq_dec (valueTy s) (TyPrim PrimUnit)
-  then
-    pure ()  (* unit is always available *)
-  else
-    st <- get ;
-    match get_value c (resources st) with
-    | None => throw (Err_Capability c CapErr_NoResourceAvailable)
-    | Some amt =>
-      let '(Token p req) := c in
-      amt' <- manager D amt req ;
-      put {| resources := set_value (Token p amt') (resources st) |}
-    end.
-
-(** [with_capability] grants a capability [C] to the evaluation of [f].
-
-    There are three results of this operation:
-
-    1. a predicate is evaluated to determine if the operation can proceed,
-       which raises an exception if not;
-
-    2. [f] is able to evaluate more permissively;
-
-    3. a resource is consumed in order to grant the capability.
-
-    (2) is easily modeled by imagining that [with_capability] introduces a
-    dynamic boolean variable (in the Lisp sense) for each capability [C] and
-    sets it to true for the scope of evaluating [f], if the predicate in (1)
-    succeeds. Later, [require_capability] tests if this boolean is true and
-    raises an exception otherwise. There is no other functionality for
-    unmanaged capabilities.
-
-    A managed capability provides the same, but in addition deducts from a
-    stateful resource after the predicate, but before defining and setting the
-    dynamic boolean. If there is not enough resource available, it raises an
-    exception. [install_capability] sets the initial amount of the
-    resource. *)
-Definition with_capability `(D : DefCap s) (c : Cap s)
-           `(f : PactM a) : PactM a :=
-  (* Check whether the capability has already been granted. If so, this
-     operation is a no-op. *)
-  env <- ask ;
-  if get_value c (granted env)
-  then
-    f
-  else
-    (* If the predicate passes, we are good to grant the capability. Note that
-       the predicate may return a list of other capabilities to be "composed"
-       with this one. *)
-    compCaps <-
-      local (λ r, {| granted := granted r
-                   ; context := InWithCapability :: context r |})
-        (predicate D c) ;
-
-    (* Note that if the resource type is unit, the only thing this function
-       could do is throw an exception. But since this is semantically
-       equivalent to throwing the same exception at the end of the predicate,
-       there is no reason to avoid this invocation in that case. *)
-    local (λ r, {| granted := granted r
-                 ; context := InWithCapability :: context r |})
-      (__claim_resource D c) ;;
-
-    (* The process of "granting" consists merely of making the capability
-       visible in the reader environment to the provided expression. *)
-    local (λ r, {| granted := existT _ _ c :: compCaps ++ granted r
-                 ; context := context r |}) f.
-
-Definition require_capability `(D : DefCap s) (c : Cap s) : PactM () :=
-  (* Note that the request resource amount must match the original
-     [with-capability] exactly.
-
-     Requiring a capability means checking whether it has been granted at any
-     point within the current scope of evaluation. *)
-  env <- ask ;
-  if get_value c (granted env)
-  then
-    pure ()
-  else
-    throw (Err_Capability c CapErr_CapabilityNotAvailable).
+Definition PactM : Type → Type := @RWSE PactEnv PactState PactLog Err.
 
 End Pact.
