src/Value.v
@@ -1,6 +1,6 @@
 Require Import
+  Coq.ZArith.ZArith
   Lib
-  Ltac
   Ty
   Exp.
 
@@ -20,14 +20,17 @@ Unset Elimination Schemes.
 (* [ValueP] is an inductive proposition that indicates whether an expression
    represents a value, i.e., that it does reduce any further. *)
 Inductive ValueP Γ : ∀ {τ}, Exp Γ τ → Prop :=
+  | LambdaP {dom cod} (e : Exp (dom :: Γ) cod) : ValueP Γ (LAM e)
   | LiteralP {ty l} : ValueP Γ (Lit (ty:=ty) l)
   | BuiltinP {τ b} : ValueP Γ (Bltn (τ:=τ) b)
+  | SymbolP {n} : ValueP Γ (Symbol n)
   | PairP {τ1 τ2} {x : Exp Γ τ1} {y : Exp Γ τ2} :
     ValueP Γ x → ValueP Γ y → ValueP Γ (Pair x y)
   | NilP {τ} : ValueP Γ (Nil (τ:=τ))
   | ConsP {τ} (x : Exp Γ τ) xs :
     ValueP Γ x → ValueP Γ xs → ValueP Γ (Cons x xs)
-  | LambdaP {dom cod} (e : Exp (dom :: Γ) cod) : ValueP Γ (LAM e).
+  | CapabilityP {tp tv} (s : Exp Γ TySym) {p : Exp Γ tp} {v : Exp Γ tv} :
+    ValueP Γ s → ValueP Γ p → ValueP Γ v → ValueP Γ (Capability s p v).
 
 Derive Signature for ValueP.
 
@@ -63,16 +66,15 @@ Lemma ValueP_dec {Γ τ} (e : Exp Γ τ) :
   ValueP Γ e ∨ ¬ ValueP Γ e.
 Proof.
   induction e; try solve [now left|now right].
-  - destruct IHe1, IHe2.
-    + now left; constructor.
-    + right; intro; inv H1; contradiction.
-    + right; intro; inv H1; contradiction.
-    + right; intro; inv H1; contradiction.
-  - destruct IHe1, IHe2.
-    + now left; constructor.
-    + right; intro; inv H1; contradiction.
-    + right; intro; inv H1; contradiction.
-    + right; intro; inv H1; contradiction.
+  - destruct IHe1, IHe2;
+    try (now left; constructor);
+    right; intro; inv H1; contradiction.
+  - destruct IHe1, IHe2;
+    try (now left; constructor);
+    right; intro; inv H1; contradiction.
+  - destruct IHe1, IHe2, IHe3;
+    try (now left; constructor);
+    right; intro; inv H2; contradiction.
 Qed.
 
 Lemma ErrorP_dec {Γ τ} (e : Exp Γ τ) :
@@ -81,14 +83,136 @@ Proof.
   induction e; solve [now left|now right].
 Qed.
 
+Inductive ValueTy : Set :=
+  | TInteger
+  | TDecimal
+  | TTime
+  | TBool
+  | TString
+  | TUnit
+  | TVoid
+  | TSymbol
+  | TList : ValueTy → ValueTy
+  | TPair : ValueTy → ValueTy → ValueTy.
+
+Derive NoConfusion NoConfusionHom Subterm EqDec for ValueTy.
+
+Inductive Value : ValueTy → Set :=
+  | VInteger      : Z → Value TInteger
+  | VDecimal      : N → Value TDecimal
+  | VTime         : nat → Value TTime
+  | VBool         : bool → Value TBool
+  | VString       : string → Value TString
+  | VUnit         : Value TUnit
+  | VSymbol       : string → Value TSymbol
+  | VList {t}     : list (Value t) → Value (TList t)
+  | VPair {t1 t2} : Value t1 → Value t2 → Value (TPair t1 t2).
+
+Derive Signature NoConfusion NoConfusionHom Subterm for Value.
+
+Equations concreteTy (τ : Ty) : ValueTy :=
+  concreteTy ℤ              := TInteger;
+  concreteTy 𝔻              := TDecimal;
+  concreteTy 𝕋              := TTime;
+  concreteTy 𝔹              := TBool;
+  concreteTy 𝕊              := TString;
+  concreteTy 𝕌              := TUnit;
+  concreteTy TySym          := TSymbol;
+  concreteTy (TyList t)     := TList (concreteTy t);
+  concreteTy (TyPair t1 t2) := TPair (concreteTy t1) (concreteTy t2);
+  concreteTy _              := TVoid.
+
+Section Value_rect.
+
+Inductive ForallT `(P : A → Type) : list A → Type :=
+    ForallT_nil : ForallT P []
+  | ForallT_cons (x : A) (l : list A) :
+    P x → ForallT P l → ForallT P (x :: l).
+
+Variable P : ∀ {t}, Value t → Type.
+
+Variable Pinteger : ∀ (num : Z), P (VInteger num).
+Variable Pdecimal : ∀ (num : N), P (VDecimal num).
+Variable Ptime    : ∀ (num : nat), P (VTime num).
+Variable Pbool    : ∀ (b : bool), P (VBool b).
+Variable Pstring  : ∀ (s : string), P (VString s).
+Variable Punit    : P VUnit.
+Variable Psym     : ∀ (sym : string), P (VSymbol sym).
+Variable Plist    : ∀ t (l : list (Value t)), ForallT P l → P (VList l).
+Variable Ppair    : ∀ t1 (x : Value t1) t2 (y : Value t2),
+                      P x → P y → P (VPair x y).
+
+Fixpoint Value_rect' `(e : Value t) : P e.
+Proof.
+  induction e.
+  - now apply Pinteger.
+  - now apply Pdecimal.
+  - now apply Ptime.
+  - now apply Pbool.
+  - now apply Pstring.
+  - now apply Punit.
+  - now apply Psym.
+  - apply Plist.
+    induction l.
+    * constructor.
+    * constructor.
+      ** now apply Value_rect'.
+      ** exact IHl.
+  - now apply Ppair.
+Qed.
+
+End Value_rect.
+
+#[export]
+Program Instance Value_EqDec {t} : EqDec (Value t).
+Next Obligation.
+  generalize dependent y.
+  dependent induction x using Value_rect'; intros;
+  dependent destruction y; subst;
+  try solve [ now left | right; congruence ];
+  try apply dec_eq_f1;
+  try (intros; now inv H).
+  - apply Z_EqDec.
+  - apply N_EqDec.
+  - apply nat_EqDec.
+  - apply bool_EqDec.
+  - apply string_EqDec.
+  - apply string_EqDec.
+  - generalize dependent l0.
+    induction l, l0; intros;
+    simpl in X.
+    + now left.
+    + right; intro; now inv H.
+    + right; intro; now inv H.
+    + inv X.
+      intuition.
+      destruct (H0 v); subst.
+      * destruct (H l0).
+        ** inv e.
+           now left.
+        ** right; intro.
+           now inv H1.
+      * right; intro.
+        now inv H1.
+  - destruct (IHx1 y1); subst.
+    + destruct (IHx2 y2); subst.
+      * now left.
+      * right; intro.
+        now inv H.
+    + right; intro.
+      now inv H.
+Defined.
+
 End Value.
 
 Arguments ValueP {Γ τ} _.
+Arguments LambdaP {Γ dom cod} _.
 Arguments LiteralP {Γ}.
 Arguments BuiltinP {Γ}.
+Arguments SymbolP {Γ}.
 Arguments PairP {Γ τ1 τ2 x y} _ _.
 Arguments NilP {Γ τ}.
 Arguments ConsP {Γ τ _ _} _ _.
-Arguments LambdaP {Γ dom cod} _.
+Arguments CapabilityP {Γ tp tv s p v} _ _ _.
 
 Arguments ErrorP {Γ τ} _.
