src/Lib.v
@@ -12,10 +12,74 @@ Require Export
   Coq.Sets.Finite_sets_facts
   Coq.Sets.Powerset_facts
   Coq.Strings.String
-  Coq.Unicode.Utf8.
+  Coq.Unicode.Utf8
+  Ltac.
+
+Require Import
+  Coq.ZArith.ZArith.
 
 From Equations Require Import Equations.
 Set Equations With UIP.
+
+Derive NoConfusion NoConfusionHom Subterm EqDec for Ascii.ascii.
+Derive NoConfusion NoConfusionHom Subterm EqDec for string.
+Derive NoConfusion NoConfusionHom Subterm EqDec for Z.
+Next Obligation. now apply Z.eq_dec. Defined.
+Derive NoConfusion NoConfusionHom Subterm EqDec for N.
+Next Obligation. now apply N.eq_dec. Defined.
+Derive NoConfusion NoConfusionHom Subterm EqDec for nat.
+Derive NoConfusion NoConfusionHom Subterm EqDec for bool.
+
+Generalizable All Variables.
+
+Lemma dec_eq_f1 `{EqDec a} (x y : a) `(f : a → b) :
+  dec_eq x y → (∀ x y, f x = f y → x = y) → dec_eq (f x) (f y).
+Proof.
+  intros.
+  destruct H0; subst.
+  - now left.
+  - right.
+    intro.
+    contradiction (H1 _ _ H0).
+Defined.
+
+Lemma dec_eq_f2 `{EqDec a} (x y : a) `{EqDec b} (z w : b) `(f : a → b → c) :
+  dec_eq x y →
+  dec_eq z w →
+  (∀ x y z w, f x z = f y w → x = y ∧ z = w) →
+  dec_eq (f x z) (f y w).
+Proof.
+  intros.
+  destruct H1, H2; subst.
+  - now left.
+  - right.
+    intro.
+    pose proof (H3 _ _ _ _ H1); reduce.
+    contradiction.
+  - right.
+    intro.
+    pose proof (H3 _ _ _ _ H1); reduce.
+    contradiction.
+  - right.
+    intro.
+    pose proof (H3 _ _ _ _ H1); reduce.
+    contradiction.
+Defined.
+
+#[export]
+Program Instance EqDec_EqDec {a} : EqDec (EqDec a).
+Next Obligation.
+  left.
+  extensionality x0.
+  extensionality y0.
+  destruct (x x0 y0); subst.
+  - destruct (y y0 y0); subst;
+    now simpl_eq.
+  - destruct (y x0 y0); subst.
+    contradiction.
+    assert (n = n0) by apply proof_irrelevance.
+    now subst.
+Defined.
 
 Corollary sum_id {X Y : Type} (e : X + Y) :
   match e with
