src/Pact/Capability.v
@@ -1,0 +1,197 @@
+Require Import
+  Coq.Arith.Arith
+  Coq.ZArith.ZArith
+  Coq.micromega.Lia
+  Coq.Strings.String
+  Hask.Control.Monad
+  Data.Monoid
+  Lib
+  Ty
+  Exp
+  Value
+  SemTy
+  Pact.
+
+Set Universe Polymorphism.
+
+From Equations Require Import Equations.
+Set Equations With UIP.
+
+Generalizable All Variables.
+
+Section Capability.
+
+Import ListNotations.
+
+Open Scope Ty_scope.
+
+(******************************************************************************
+ * Capabilities
+ *)
+
+Record DefCap (s : CapSig) : Type := {
+  predicate : Cap s → PactM (list { s : CapSig & Cap s });
+  manager   : Value (valueTy s) → Value (valueTy s) → PactM (Value (valueTy s))
+}.
+
+Derive NoConfusion NoConfusionHom Subterm for DefCap.
+
+Arguments predicate {_} _ _.
+Arguments manager {_} _ _.
+
+Import EqNotations.
+
+Definition get_value `(c : Cap s) (l : list { s : CapSig & Cap s }) :
+  option (Value (valueTy s)) :=
+  let '(Token n arg _) := c in
+  let fix go (l : list { s : CapSig & Cap s }) :
+    option (Value (valueTy s)) :=
+    match l with
+    | [] => None
+    | existT _ s' (Token n' arg' val') :: xs =>
+        match eq_dec s s' with
+        | left Hs =>
+            match eq_dec n n' with
+            | left _ =>
+                match eq_dec arg
+                        (rew <- [λ x, Value (paramTy x)] Hs in arg') with
+                | left _ =>
+                    Some (rew <- [λ x, Value (valueTy x)] Hs in val')
+                | _ => go xs
+                end
+            | _ => go xs
+            end
+        | _ => go xs
+        end
+    end
+  in go l.
+
+Definition set_value `(c : Cap s) (l : list { s : CapSig & Cap s }) :
+  list { s : CapSig & Cap s } :=
+  let '(Token n arg _) := c in
+  let fix go (l : list { s : CapSig & Cap s }) :
+    list { s : CapSig & Cap s } :=
+    match l with
+    | [] => []
+    | existT _ s' (Token n' arg' _) :: xs =>
+        match eq_dec s s' with
+        | left Hs =>
+            match eq_dec n n' with
+            | left _ =>
+                match eq_dec arg
+                        (rew <- [λ x, Value (paramTy x)] Hs in arg') with
+                | left _ => existT _ s c :: go xs
+                | _ => go xs
+                end
+            | _ => go xs
+            end
+        | _ => go xs
+        end
+    end
+  in go l.
+
+(* The functions below all take a [DefCap] because name resolution must happen
+   in the parser, since capability predicates can themselves refer to the
+   current module. *)
+
+(* "Installing" a capability assigns a resource amount associated with that
+   capability, to be consumed by future calls to [with-capability].
+
+   Note that a capability can be installed either by the user calling
+   [install-capability] directly, or by the chain calling this function if it
+   sees a signed capability as part of a transaction. *)
+Definition install_capability (c : Cap s) : PactM () :=
+  env <- ask ;
+  if in_dec EvalContext_EqDec InWithCapability (context env)
+  then
+    throw (Err_Capability c CapErr_CannotInstallDuringWith)
+  else
+    modify (λ st, {| resources := set_value c (resources st) |}).
+
+Definition __claim_resource `(D : DefCap s) (c : Cap s) : PactM () :=
+  (* Check the current amount of resource associated with this capability, and
+     whether the requested amount is available. If so, update the available
+     amount. Note: unit is used to represent unmanaged capabilities. *)
+  if eq_dec (valueTy s) TUnit
+  then
+    pure ()  (* unit is always available *)
+  else
+    st <- get ;
+    match get_value c (resources st) with
+    | None => throw (Err_Capability c CapErr_NoResourceAvailable)
+    | Some amt =>
+      let '(Token n p req) := c in
+      amt' <- manager D amt req ;
+      put {| resources := set_value (Token n p amt') (resources st) |}
+    end.
+
+(** [with_capability] grants a capability [C] to the evaluation of [f].
+
+    There are three results of this operation:
+
+    1. a predicate is evaluated to determine if the operation can proceed,
+       which raises an exception if not;
+
+    2. [f] is able to evaluate more permissively;
+
+    3. a resource is consumed in order to grant the capability.
+
+    (2) is easily modeled by imagining that [with_capability] introduces a
+    dynamic boolean variable (in the Lisp sense) for each capability [C] and
+    sets it to true for the scope of evaluating [f], if the predicate in (1)
+    succeeds. Later, [require_capability] tests if this boolean is true and
+    raises an exception otherwise. There is no other functionality for
+    unmanaged capabilities.
+
+    A managed capability provides the same, but in addition deducts from a
+    stateful resource after the predicate, but before defining and setting the
+    dynamic boolean. If there is not enough resource available, it raises an
+    exception. [install_capability] sets the initial amount of the
+    resource. *)
+Definition with_capability `(D : DefCap s) (c : Cap s)
+           `(f : PactM a) : PactM a :=
+  (* Check whether the capability has already been granted. If so, this
+     operation is a no-op. *)
+  env <- ask ;
+  if get_value c (granted env)
+  then
+    f
+  else
+    (* jww (2022-07-19): This can only be executed within the module that
+       declares the capability. *)
+
+    (* If the predicate passes, we are good to grant the capability. Note that
+       the predicate may return a list of other capabilities to be "composed"
+       with this one. *)
+    compCaps <-
+      local (λ r, {| granted := granted r
+                   ; context := InWithCapability :: context r |})
+        (predicate D c) ;
+
+    (* Note that if the resource type is unit, the only thing this function
+       could do is throw an exception. But since this is semantically
+       equivalent to throwing the same exception at the end of the predicate,
+       there is no reason to avoid this invocation in that case. *)
+    local (λ r, {| granted := granted r
+                 ; context := InWithCapability :: context r |})
+      (__claim_resource D c) ;;
+
+    (* The process of "granting" consists merely of making the capability
+       visible in the reader environment to the provided expression. *)
+    local (λ r, {| granted := existT _ _ c :: compCaps ++ granted r
+                 ; context := context r |}) f.
+
+Definition require_capability (c : Cap s) : PactM () :=
+  (* Note that the request resource amount must match the original
+     [with-capability] exactly.
+
+     Requiring a capability means checking whether it has been granted at any
+     point within the current scope of evaluation. *)
+  env <- ask ;
+  if get_value c (granted env)
+  then
+    pure ()
+  else
+    throw (Err_Capability c CapErr_CapabilityNotAvailable).
+
+End Capability.
