src/SemExp.v
@@ -1,0 +1,200 @@
+Require Import
+  Coq.ZArith.ZArith
+  Hask.Control.Monad
+  Hask.Data.Either
+  ilist
+  Lib
+  Ty
+  Exp
+  Value
+  Ren
+  Sub
+  SemTy
+  Pact
+  Pact.Capability.
+
+From Equations Require Import Equations.
+
+Generalizable All Variables.
+
+Section SemExp.
+
+Import ListNotations.
+
+Definition SemEnv Γ : Type := ilist (SemTy (m:=PactM)) Γ.
+
+Fixpoint SemVar `(v : Var Γ τ) : SemEnv Γ → SemTy τ :=
+  match v with
+  | ZV   => λ se, fst se
+  | SV v => λ se, SemVar v (snd se)
+  end.
+
+Equations RenSem {Γ Γ'} (r : Ren Γ Γ') (se : SemEnv Γ) : SemEnv Γ' :=
+  RenSem NoRen    se      := se;
+  RenSem (Drop r) (_, se) := RenSem r se;
+  RenSem (Keep r) (e, se) := (e, RenSem r se).
+
+Lemma RenSem_inil (r : Ren [] []) :
+  RenSem r () = ().
+Proof. now dependent destruction r. Qed.
+
+Lemma RenSem_idRen {Γ} (se : SemEnv Γ) :
+  RenSem idRen se = se.
+Proof.
+  induction Γ; destruct se; simpl; simp RenSem; intros; auto.
+  now rewrite IHΓ.
+Qed.
+
+Lemma RenSem_skip1 {Γ τ} (e : SemTy τ) (se : SemEnv Γ) :
+  RenSem skip1 (e, se) = se.
+Proof.
+  induction Γ; destruct se; simpl; intros; auto.
+  unfold skip1; simp RenSem.
+  now rewrite RenSem_idRen.
+Qed.
+
+Lemma SemVar_RenSem Γ τ (v : Var Γ τ) Γ' (r : Ren Γ' Γ) (se : SemEnv Γ') :
+  SemVar v (RenSem r se) = SemVar (RenVar r v) se.
+Proof.
+  intros.
+  induction r; simp RenSem; simp RenVar; simpl;
+  destruct se; simp RenSem; auto.
+  now dependent elimination v; simpl; simp RenVar.
+Qed.
+
+Lemma RenSem_RcR {Γ Γ' Γ''} (f : Ren Γ' Γ'') (g : Ren Γ Γ') (se : SemEnv Γ) :
+  RenSem (RcR f g) se = RenSem f (RenSem g se).
+Proof.
+  generalize dependent Γ''.
+  generalize dependent Γ'.
+  induction Γ; destruct se; simpl; intros; auto.
+  - inversion g; subst.
+    rewrite RenSem_inil.
+    inversion f; subst.
+    now rewrite !RenSem_inil.
+  - dependent elimination g; simp RenSem.
+    + now rewrite <- IHΓ; simp RcR; simp RenSem.
+    + dependent elimination f; simp RenSem;
+      now rewrite <- IHΓ; simp RcR; simp RenSem.
+Qed.
+
+Definition liftJoin2 `{Monad m} `(f : a -> b -> m c)
+           (ma : m a) (mb : m b) : m c :=
+   join (liftA2 f ma mb).
+
+Notation "f =<< x" := (x >>= f) (at level 42, right associativity).
+
+Program Fixpoint SemExp `(e : Exp Γ τ) : SemEnv Γ → PactM (SemTy τ) :=
+  match e with
+  | VAR v         => λ se, pure (SemVar v se)
+  | LAM e         => λ se, pure (λ x, SemExp e (x, se))
+  | APP e1 e2     => λ se, liftJoin2 (m:=PactM) id (SemExp e1 se) (SemExp e2 se)
+
+  | Error e       => λ _,  throw (Err_Exp e)
+  | Lit l         => λ _,  throw (Err_Exp Err_CarNil) (* jww (2022-07-18): TODO *)
+  | Bltn b        => λ _,  throw (Err_Exp Err_CarNil) (* jww (2022-07-18): TODO *)
+  | Symbol n      => λ _,  pure n
+  | If b t e      => λ se, b' <- SemExp b se ;
+                           if b' : bool
+                           then SemExp t se
+                           else SemExp e se
+  | Pair x y      => λ se, liftA2 pair (SemExp x se) (SemExp y se)
+  | Fst p         => λ se, fst <$> SemExp p se
+  | Snd p         => λ se, snd <$> SemExp p se
+  | Nil           => λ se, pure nil
+  | Cons x xs     => λ se, x'  <- SemExp x se ;
+                           xs' <- SemExp xs se ;
+                           pure (x' :: xs')
+  | Car xs        => λ se, xs' <- SemExp xs se ;
+                           match xs' with
+                           | []     => throw (Err_Exp Err_CarNil)
+                           | x :: _ => pure x
+                           end
+  | Cdr xs        => λ se, xs' <- SemExp xs se ;
+                           match xs' with
+                           | []      => throw (Err_Exp Err_CdrNil)
+                           | _ :: xs => pure xs
+                           end
+  | IsNil xs      => λ se, xs' <- SemExp xs se ;
+                           match xs' with
+                           | []      => pure true
+                           | _ :: xs => pure false
+                           end
+  | Seq exp1 exp2 => λ se, SemExp exp1 se >> SemExp exp2 se
+
+  | @Capability _ tp tv n p v => λ se,
+      match Concreteness tp with
+      | Some Hp =>
+          match Concreteness tv with
+          | Some Hv =>
+              n' <- SemExp n se ;
+              p' <- SemExp p se ;
+              v' <- SemExp v se ;
+              pure (Token n' (concrete Hp p') (concrete Hv v'))
+          | None => throw (Err_Exp Err_CarNil) (* jww (2022-07-19): TODO *)
+          end
+      | None => throw (Err_Exp Err_CarNil) (* jww (2022-07-19): TODO *)
+      end
+
+  | InstallCapability c => λ se, install_capability _ =<< SemExp c se
+  | WithCapability c e  => λ se,
+      c' <- SemExp c se ;
+      with_capability _ c' (SemExp e se)
+  | RequireCapability c => λ se, require_capability _ =<< SemExp c se
+  end.
+
+Definition sem `(e : Exp [] τ) : Err + SemTy τ := SemExp e tt.
+Arguments sem {_} _ /.
+
+Lemma SemExp_RenSem {Γ Γ' τ} (e : Exp Γ τ) (r : Ren Γ' Γ) (se : SemEnv Γ') :
+  SemExp e (RenSem r se) = SemExp (RenExp r e) se.
+Proof.
+  generalize dependent Γ'.
+  induction e; simpl; intros; auto.
+  - rewrite IHe1; repeat f_equal.
+    extensionality b.
+    now destruct b; simpl.
+  - rewrite IHe2; repeat f_equal.
+    now apply IHe1.
+  - now rewrite IHe.
+  - now rewrite IHe.
+  - now rewrite IHe1, IHe2.
+  - now rewrite IHe.
+  - now rewrite IHe.
+  - now rewrite IHe.
+  - now rewrite IHe1, IHe2.
+  - now rewrite SemVar_RenSem.
+  - f_equal.
+    extensionality z.
+    fold SemTy in z.
+    rewrite <- IHe; clear IHe.
+    simpl.
+    now repeat f_equal.
+  - now rewrite IHe1, IHe2.
+Qed.
+
+Lemma SemExp_wk `(E : SemEnv Γ) {τ τ'} (y : SemTy τ') (e : Exp Γ τ) :
+  SemExp (wk e) (y, E) = SemExp e E.
+Proof.
+  unfold wk.
+  rewrite <- SemExp_RenSem; simpl.
+  f_equal.
+  now rewrite RenSem_skip1.
+Qed.
+
+Lemma SemExp_ValueP {Γ τ} (e : Exp Γ τ) (se : SemEnv Γ) :
+  ValueP e → ∃ x, SemExp e se = pure x.
+Proof.
+  induction 1; simpl; intros;
+  try (now eexists; eauto); reduce.
+  - admit.                      (* jww (2022-07-18): TODO *)
+  - admit.                      (* jww (2022-07-18): TODO *)
+  - exists (x1, x0).
+    now rewrite H1, H2; simpl.
+  - exists (x1 :: x0).
+    now rewrite H1, H2; simpl.
+Abort.
+
+End SemExp.
+
+Notation "f =<< x" := (x >>= f) (at level 42, right associativity).
