src/SemTy.v
@@ -1,0 +1,159 @@
+Require Import
+  Coq.ZArith.ZArith
+  Hask.Control.Monad
+  Hask.Data.Either
+  ilist
+  Lib
+  Ty
+  Exp
+  Value
+  Ren
+  Sub.
+
+From Equations Require Import Equations.
+Set Equations With UIP.
+
+Generalizable All Variables.
+
+Section SemTy.
+
+Import ListNotations.
+
+Definition SemPrimType (ty : PrimType) : Set :=
+  match ty with
+  | PrimInteger => Z
+  | PrimDecimal => N
+  | PrimTime    => nat
+  | PrimBool    => bool
+  | PrimString  => string
+  | PrimUnit    => unit
+  end.
+
+Record CapSig : Set := {
+  paramTy : ValueTy;
+  valueTy : ValueTy;
+}.
+
+Derive NoConfusion NoConfusionHom Subterm EqDec for CapSig.
+
+Inductive Cap (s : CapSig) : Set :=
+  | Token (name : string) : Value (paramTy s) → Value (valueTy s) → Cap s.
+
+Derive NoConfusion NoConfusionHom Subterm EqDec for Cap.
+
+Arguments Token {s} name arg val.
+
+Definition nameOf `(c : Cap s) : string :=
+  match c with Token n _ _ => n end.
+
+Definition paramOf `(c : Cap s) : Value (paramTy s) :=
+  match c with Token _ p _ => p end.
+
+Definition valueOf `(c : Cap s) : Value (valueTy s) :=
+  match c with Token _ _ v => v end.
+
+Context `{Monad m}.
+
+Fixpoint SemTy (τ : Ty) : Type :=
+  match τ with
+  | TyArrow dom cod => SemTy dom → m (SemTy cod)
+
+  | TyPrim ty       => SemPrimType ty
+  | TySym           => string
+  | TyList τ        => list (SemTy τ)
+  | TyPair t1 t2    => SemTy t1 * SemTy t2
+
+  | TyCap p v       => Cap {| paramTy := concreteTy p
+                            ; valueTy := concreteTy v |}
+  end.
+
+Notation "⟦ t ⟧" := (SemTy t) (at level 9) : type_scope.
+
+Equations concrete {τ} (H : ConcreteP τ) (e : ⟦τ⟧) : Value (concreteTy τ) :=
+  concrete (τ:=ℤ)        PrimDecP     lit := VInteger lit;
+  concrete (τ:=𝔻)        PrimDecP     lit := VDecimal lit;
+  concrete (τ:=𝕋)        PrimDecP     lit := VTime lit;
+  concrete (τ:=𝔹)        PrimDecP     lit := VBool lit;
+  concrete (τ:=𝕊)        PrimDecP     lit := VString lit;
+  concrete (τ:=𝕌)        PrimDecP     tt  := VUnit;
+  concrete (τ:=TySym)    SymDecP      sym := VSymbol sym;
+  concrete (τ:=TyList t) (ListDecP H) xs  := VList (map (concrete H) xs);
+  concrete (τ:=TyPair t1 t2) (PairDecP Hx Hy) (x, y) :=
+    VPair (concrete Hx x) (concrete Hy y).
+
+Equations Concrete_EqDec {t} (H : ConcreteP t) : EqDec ⟦t⟧ :=
+  Concrete_EqDec (t:=TyPrim PrimUnit) _ tt tt := left _;
+  Concrete_EqDec (t:=TyPrim PrimString) _ s1 s2
+    with eq_dec s1 s2 := {
+      | left _  => left _
+      | right _ => right _
+    };
+  Concrete_EqDec (t:=TyPrim PrimInteger) _ i1 i2
+    with eq_dec i1 i2 := {
+      | left _  => left _
+      | right _ => right _
+    };
+  Concrete_EqDec (t:=TyPrim PrimDecimal) _ d1 d2
+    with eq_dec d1 d2 := {
+      | left _  => left _
+      | right _ => right _
+    };
+  Concrete_EqDec (t:=TyPrim PrimBool) _ b1 b2
+    with eq_dec b1 b2 := {
+      | left _  => left _
+      | right _ => right _
+    };
+  Concrete_EqDec (t:=TyPrim PrimTime) _ t1 t2
+    with eq_dec t1 t2 := {
+      | left _  => left _
+      | right _ => right _
+    };
+
+  Concrete_EqDec (t:=TySym) _ n1 n2 := eq_dec n1 n2;
+
+  Concrete_EqDec (t:=TyList _)  _ ([]) ([]) := left _;
+  Concrete_EqDec (t:=TyList _)  _ (_ :: _) ([]) := right _;
+  Concrete_EqDec (t:=TyList _)  _ ([]) (_ :: _) := right _;
+  Concrete_EqDec (t:=TyList ty) (ListDecP H) (x1 :: xs1) (x2 :: xs2)
+    with @eq_dec _ (Concrete_EqDec (t:=ty) H) x1 x2 := {
+      | left _
+        with @eq_dec _ (list_eqdec (Concrete_EqDec (t:=ty) H)) xs1 xs2 := {
+        | left _  => left _
+        | right _ => right _
+      }
+      | right _ => right _
+    };
+
+  Concrete_EqDec (t:=TyPair t1 t2) (PairDecP H1 H2) (x1, y1) (x2, y2)
+    with @eq_dec _ (Concrete_EqDec (t:=t1) H1) x1 x2 := {
+      | left  _ with @eq_dec _ (Concrete_EqDec (t:=t2) H2) y1 y2 := {
+        | left _  => left _
+        | right _ => right _
+      }
+      | right _ => right _
+    }.
+
+#[export]
+Instance Concrete_EqDec' {t} : ConcreteP t → EqDec ⟦t⟧ :=
+  Concrete_EqDec (t:=t).
+
+Inductive Value t : Type :=
+  | Bundle : ConcreteP t → ⟦t⟧ → Value t.
+
+Derive NoConfusion NoConfusionHom Subterm EqDec for Value.
+Next Obligation.
+  destruct x, y.
+  destruct (eq_dec c c0); subst.
+  - destruct (@eq_dec _ (Concrete_EqDec c0) s s0); subst.
+    + now left.
+    + right; intro.
+      now inv H0.
+  - pose proof (ConcreteP_irrelevance c c0).
+    contradiction.
+Defined.
+
+End SemTy.
+
+Arguments Token {s} name arg val.
+
+Notation "⟦ t ⟧" := (SemTy t) (at level 9) : type_scope.
